add binary search example and tweak instrs.v file

examples/binary_search.c
@@ -1,0 +1,26 @@
+#include <stddef.h>
+#include <stdbool.h>
+
+// compiled with armv8-a clang 11.0.1
+// options: -O2
+// https://godbolt.org/z/sEGvPoPox
+
+typedef bool (*comp_fn)(void *, void *);
+
+size_t binary_search(comp_fn comp, void **xs, size_t n, void *x) {
+  size_t l = 0, r = n;
+  while(l < r) {
+    size_t k = l + (r - l) / 2;
+    if (comp(xs[k], x)) {
+      l = k + 1;
+    } else {
+      r = k;
+    }
+  }
+  return l;
+}
+
+bool compare_int(void *x, void *y) {
+  size_t *xi = x, *yi = y;
+  return *xi <= *yi;
+}
