examples/binary_search.s
@@ -1,0 +1,39 @@
+binary_search:                          // @binary_search
+        stp     x29, x30, [sp, #-64]!           // 16-byte Folded Spill
+        stp     x24, x23, [sp, #16]             // 16-byte Folded Spill
+        stp     x22, x21, [sp, #32]             // 16-byte Folded Spill
+        stp     x20, x19, [sp, #48]             // 16-byte Folded Spill
+        mov     x29, sp
+        cbz     x2, .LBB0_3
+        mov     x19, x3
+        mov     x20, x2
+        mov     x21, x1
+        mov     x22, x0
+        mov     x23, xzr
+.LBB0_2:                                // =>This Inner Loop Header: Depth=1
+        sub     x8, x20, x23
+        add     x24, x23, x8, lsr #1
+        ldr     x0, [x21, x24, lsl #3]
+        mov     x1, x19
+        blr     x22
+        tst     w0, #0x1
+        csel    x20, x20, x24, ne
+        csinc   x23, x23, x24, eq
+        cmp     x20, x23
+        b.hi    .LBB0_2
+        b       .LBB0_4
+.LBB0_3:
+        mov     x23, xzr
+.LBB0_4:
+        mov     x0, x23
+        ldp     x20, x19, [sp, #48]             // 16-byte Folded Reload
+        ldp     x22, x21, [sp, #32]             // 16-byte Folded Reload
+        ldp     x24, x23, [sp, #16]             // 16-byte Folded Reload
+        ldp     x29, x30, [sp], #64             // 16-byte Folded Reload
+        ret
+compare_int:                            // @compare_int
+        ldr     x8, [x0]
+        ldr     x9, [x1]
+        cmp     x8, x9
+        cset    w0, ls
+        ret
