instructions/binary_search/a3c.v
@@ -1,23 +1,28 @@
 From isla Require Import isla_lang.
 
-Definition a743c : list trc := [
+Definition a3c : list trc := [
   [
     Smt (DeclareConst 49%Z (Ty_BitVec 64%N)) Mk_annot;
-    ReadReg "R5" [] (Val_Symbolic 49%Z) Mk_annot;
+    ReadReg "R22" [] (Val_Symbolic 49%Z) Mk_annot;
     Smt (DefineConst 50%Z (Val (Val_Symbolic 49%Z) Mk_annot)) Mk_annot;
-    ReadReg "InGuardedPage" [] (Val_Bool false) Mk_annot;
+    MarkReg "R22" "ignore_edge" Mk_annot;
+    MarkReg "R30" "ignore_edge" Mk_annot;
+    Smt (DeclareConst 51%Z (Ty_BitVec 64%N)) Mk_annot;
+    ReadReg "_PC" [] (Val_Symbolic 51%Z) Mk_annot;
+    Smt (DefineConst 53%Z (Manyop (Bvmanyarith Bvadd) [Val (Val_Symbolic 51%Z) Mk_annot; Val (Val_Bits [BV{64%N} 0x4%Z]) Mk_annot] Mk_annot)) Mk_annot;
+    WriteReg "R30" [] (Val_Symbolic 53%Z) Mk_annot;
     ReadReg "PSTATE" [Field "nRW"] (Val_Struct [("nRW", Val_Bits [BV{1%N} 0x0%Z])]) Mk_annot;
     ReadReg "CFG_ID_AA64PFR0_EL1_EL0" [] (Val_Bits [BV{4%N} 0x1%Z]) Mk_annot;
     ReadReg "CFG_ID_AA64PFR0_EL1_EL1" [] (Val_Bits [BV{4%N} 0x1%Z]) Mk_annot;
     ReadReg "CFG_ID_AA64PFR0_EL1_EL2" [] (Val_Bits [BV{4%N} 0x1%Z]) Mk_annot;
     ReadReg "CFG_ID_AA64PFR0_EL1_EL3" [] (Val_Bits [BV{4%N} 0x1%Z]) Mk_annot;
-    Smt (DefineConst 51%Z (Val (Val_Symbolic 50%Z) Mk_annot)) Mk_annot;
-    BranchAddress (Val_Symbolic 51%Z) Mk_annot;
-    Smt (DefineConst 52%Z (Val (Val_Symbolic 50%Z) Mk_annot)) Mk_annot;
+    Smt (DefineConst 54%Z (Val (Val_Symbolic 50%Z) Mk_annot)) Mk_annot;
+    BranchAddress (Val_Symbolic 54%Z) Mk_annot;
+    Smt (DefineConst 55%Z (Val (Val_Symbolic 50%Z) Mk_annot)) Mk_annot;
     ReadReg "PSTATE" [Field "EL"] (Val_Struct [("EL", Val_Bits [BV{2%N} 0x2%Z])]) Mk_annot;
     ReadReg "SCR_EL3" [] (Val_Bits [BV{32%N} 0x0%Z]) Mk_annot;
     ReadReg "TCR_EL2" [] (Val_Bits [BV{64%N} 0x0%Z]) Mk_annot;
-    WriteReg "_PC" [] (Val_Symbolic 52%Z) Mk_annot;
+    WriteReg "_PC" [] (Val_Symbolic 55%Z) Mk_annot;
     WriteReg "__PC_changed" [] (Val_Bool true) Mk_annot
   ]
 ].
