examples/binary_search.v
@@ -1,0 +1,99 @@
+Require Import isla.base.
+Require Import isla.opsem.
+Require Import isla.automation.
+Require Import isla.adequacy.
+Require Import isla.examples.sys_regs.
+From isla.instructions.binary_search Require Import instrs.
+
+
+(*
+The code can be generated with
+PATH=$PWD/bin:$PATH dune exec -- isla-coq examples/binary_search.dump -d -o instructions/binary_search  -n "a{addr}" --coqdir=isla.instructions.binary_search
+
+*)
+
+Definition binary_search_loop_spec `{!islaG Σ} `{!threadG} : iProp Σ :=
+  ∃ (tmp src dst i n : bv 64) (srcdata dstdata : list byte) (pstaten pstatez pstatec pstatev : bv 1),
+  reg_col sys_regs ∗
+  "PSTATE" # "N" ↦ᵣ Val_Bits pstaten ∗ "PSTATE" # "Z" ↦ᵣ Val_Bits pstatez ∗
+  "PSTATE" # "C" ↦ᵣ Val_Bits pstatec ∗ "PSTATE" # "V" ↦ᵣ Val_Bits pstatev ∗
+  "R0" ↦ᵣ Val_Bits dst ∗ "R1" ↦ᵣ Val_Bits src ∗ "R2" ↦ᵣ Val_Bits n ∗
+  "R3" ↦ᵣ Val_Bits i ∗ "R4" ↦ᵣ Val_Bits tmp ∗
+  src ↦ₘ∗ srcdata ∗ dst ↦ₘ∗ dstdata ∗
+  instr_pre 0x0000000010300054 (
+    ∃ (tmp n : bv 64) (pstaten pstatez pstatec pstatev : bv 1),
+      reg_col sys_regs ∗
+      "PSTATE" # "N" ↦ᵣ Val_Bits pstaten ∗ "PSTATE" # "Z" ↦ᵣ Val_Bits pstatez ∗
+      "PSTATE" # "C" ↦ᵣ Val_Bits pstatec ∗ "PSTATE" # "V" ↦ᵣ Val_Bits pstatev ∗
+      "R0" ↦ᵣ Val_Bits dst ∗ "R1" ↦ᵣ Val_Bits src ∗ "R2" ↦ᵣ Val_Bits n ∗
+      "R4" ↦ᵣ Val_Bits tmp ∗ "R3" ↦ᵣ Val_Bits n ∗
+      src ↦ₘ∗ srcdata ∗ dst ↦ₘ∗ srcdata ∗
+      True
+  )
+.
+
+Arguments binary_search_loop_spec /.
+
+Lemma binary_search_loop `{!islaG Σ} `{!threadG} :
+  instr 0x000000001030002c (Some a2c) -∗
+  instr 0x0000000010300030 (Some a30) -∗
+  instr 0x0000000010300034 (Some a34) -∗
+  instr 0x0000000010300038 (Some a38) -∗
+  instr 0x000000001030003c (Some a3c) -∗
+  instr 0x0000000010300040 (Some a40) -∗
+  instr 0x0000000010300044 (Some a44) -∗
+  instr 0x0000000010300048 (Some a48) -∗
+  instr 0x000000001030004c (Some a4c) -∗
+  instr 0x0000000010300050 (Some a50) -∗
+  □ instr_pre 0x000000001030002c binary_search_loop_spec -∗
+  instr_body 0x000000001030002c binary_search_loop_spec.
+Proof.
+  iStartProof.
+  Time repeat liAStep; liShow.
+Abort.
+
+Lemma binary_search `{!islaG Σ} `{!threadG} :
+  instr 0x0000000010300000 (Some a0) -∗
+  instr 0x0000000010300004 (Some a4) -∗
+  instr 0x0000000010300008 (Some a8) -∗
+  instr 0x000000001030000c (Some ac) -∗
+  instr 0x0000000010300010 (Some a10) -∗
+  instr 0x0000000010300014 (Some a14) -∗
+  instr 0x0000000010300018 (Some a18) -∗
+  instr 0x000000001030001c (Some a1c) -∗
+  instr 0x0000000010300020 (Some a20) -∗
+  instr 0x0000000010300024 (Some a24) -∗
+  instr 0x0000000010300028 (Some a28) -∗
+
+  instr 0x0000000010300054 (Some a54) -∗
+  instr 0x0000000010300058 (Some a58) -∗
+  instr 0x000000001030005c (Some a5c) -∗
+  instr 0x0000000010300060 (Some a60) -∗
+  instr 0x0000000010300064 (Some a64) -∗
+  instr 0x0000000010300068 (Some a68) -∗
+  instr 0x000000001030006c (Some a6c) -∗
+  instr 0x0000000010300070 (Some a70) -∗
+  □ instr_pre 0x000000001030002c binary_search_loop_spec -∗
+  instr_body 0x0000000010300000 (
+    ∃ (tmp1 tmp2 src dst n ret : bv 64) (srcdata dstdata : list byte) (pstaten pstatez pstatec pstatev : bv 1),
+    reg_col sys_regs ∗
+    "PSTATE" # "N" ↦ᵣ Val_Bits pstaten ∗ "PSTATE" # "Z" ↦ᵣ Val_Bits pstatez ∗
+    "PSTATE" # "C" ↦ᵣ Val_Bits pstatec ∗ "PSTATE" # "V" ↦ᵣ Val_Bits pstatev ∗
+    "R0" ↦ᵣ Val_Bits dst ∗ "R1" ↦ᵣ Val_Bits src ∗ "R2" ↦ᵣ Val_Bits n ∗
+    "R3" ↦ᵣ Val_Bits tmp2 ∗ "R4" ↦ᵣ Val_Bits tmp1 ∗
+    "R30" ↦ᵣ Val_Bits ret ∗
+    instr_pre (bv_unsigned ret) (
+    ∃ (tmp1 tmp2 n : bv 64) (pstaten pstatez pstatec pstatev : bv 1),
+      reg_col sys_regs ∗
+      "PSTATE" # "N" ↦ᵣ Val_Bits pstaten ∗ "PSTATE" # "Z" ↦ᵣ Val_Bits pstatez ∗
+      "PSTATE" # "C" ↦ᵣ Val_Bits pstatec ∗ "PSTATE" # "V" ↦ᵣ Val_Bits pstatev ∗
+      "R0" ↦ᵣ Val_Bits dst ∗ "R1" ↦ᵣ Val_Bits src ∗ "R2" ↦ᵣ Val_Bits n ∗
+      "R3" ↦ᵣ Val_Bits tmp2 ∗ "R4" ↦ᵣ Val_Bits tmp1 ∗
+      "R30" ↦ᵣ Val_Bits ret ∗
+      src ↦ₘ∗ srcdata ∗ dst ↦ₘ∗ srcdata ∗
+      True
+  )).
+Proof.
+  iStartProof.
+  Time repeat liAStep; liShow.
+Abort.
