instructions/binary_search/a24.v
@@ -1,0 +1,10 @@
+From isla Require Import isla_lang.
+
+Definition a24 : list trc := [
+  [
+    Smt (DeclareConst 48%Z (Ty_BitVec 64%N)) Mk_annot;
+    ReadReg "R0" [] (Val_Symbolic 48%Z) Mk_annot;
+    Smt (DefineConst 54%Z (Manyop (Bvmanyarith Bvor) [Val (Val_Bits [BV{64%N} 0x0%Z]) Mk_annot; Val (Val_Symbolic 48%Z) Mk_annot] Mk_annot)) Mk_annot;
+    WriteReg "R22" [] (Val_Symbolic 54%Z) Mk_annot
+  ]
+].
